examples/cnf/array/ccnf_parseProgScript.sml
@@ -1,0 +1,222 @@
+(*
+  Adds file-level parsing and formula construction to ccnf_arrayProg
+*)
+Theory ccnf_parseProg
+Ancestors
+  ccnf ccnf_list ccnf_arrayProg mlint syntax_helper
+Libs
+  preamble basis
+
+val _ = hide_environments true;
+
+val _ = translation_extends"ccnf_arrayProg";
+
+(* Reported by the file-level entry points *)
+Definition format_dimacs_failure_def:
+  format_dimacs_failure (lno:num) s =
+  «c DIMACS parse failed at line: » ^ toString lno ^ «. Reason: » ^ s ^ «\n»
+End
+
+val res = translate format_dimacs_failure_def;
+
+Definition notfound_string_def:
+  notfound_string f =
+  concat[«c Input file: »; f; « no such file or directory\n»]
+End
+
+val res = translate notfound_string_def;
+
+(* Parsing helpers *)
+
+(* TODO: Mostly copied from mlintTheory *)
+val result = translate (fromChar_unsafe_def |> REWRITE_RULE [GSYM ml_translatorTheory.sub_check_def]);
+
+Definition fromChars_range_unsafe_tail_def:
+  fromChars_range_unsafe_tail b n str mul acc =
+  if n ≤ b then acc
+  else
+    let m = n - 1 in
+    fromChars_range_unsafe_tail b m str (mul * 10)
+      (acc + fromChar_unsafe (strsub str m) * mul)
+Termination
+  WF_REL_TAC`measure (λ(b,n,_). n)`>>
+  rw[]
+End
+
+Theorem fromChars_range_unsafe_tail_eq:
+  ∀n l s mul acc.
+  fromChars_range_unsafe_tail l (n+l) s mul acc =
+  (fromChars_range_unsafe l n s) * mul + acc
+Proof
+  Induct
+  >-
+    rw[Once fromChars_range_unsafe_tail_def,fromChars_range_unsafe_def]>>
+  rw[]>>
+  simp[Once fromChars_range_unsafe_tail_def,ADD1,fromChars_range_unsafe_def]>>
+  fs[ADD1]
+QED
+
+Theorem fromChars_range_unsafe_alt:
+  fromChars_range_unsafe l n s =
+  fromChars_range_unsafe_tail l (n+l) s 1 0
+Proof
+  rw[fromChars_range_unsafe_tail_eq]
+QED
+
+val result = translate fromChars_range_unsafe_tail_def;
+
+val fromchars_range_unsafe_tail_side_def = theorem"fromchars_range_unsafe_tail_side_def";
+
+Theorem fromchars_range_unsafe_tail_side_def[allow_rebind]:
+  ∀a1 a0 a2 a3 a4.
+  fromchars_range_unsafe_tail_side a0 a1 a2 a3 a4 ⇔
+   ¬(a1 ≤ a0) ⇒
+   (T ∧ a1 < 1 + strlen a2 ∧ 0 < strlen a2) ∧
+   fromchars_range_unsafe_tail_side a0 (a1 − 1) a2 (a3 * 10)
+     (a4 + fromChar_unsafe (strsub a2 (a1 − 1)) * a3)
+Proof
+  Induct>>
+  rw[Once fromchars_range_unsafe_tail_side_def]>>
+  simp[]>>eq_tac>>rw[ADD1]>>
+  gvs[]
+QED
+
+val result = translate fromChars_range_unsafe_alt;
+
+val res = translate_no_ind (mlintTheory.fromChars_unsafe_def
+  |> REWRITE_RULE[maxSmall_DEC_def,padLen_DEC_eq]);
+
+Theorem fromChars_unsafe_ind[local]:
+  fromchars_unsafe_ind
+Proof
+  rewrite_tac [fetch "-" "fromchars_unsafe_ind_def"]
+  \\ rpt gen_tac
+  \\ rpt (disch_then strip_assume_tac)
+  \\ match_mp_tac (latest_ind ())
+  \\ rpt strip_tac
+  \\ last_x_assum match_mp_tac
+  \\ rpt strip_tac
+  \\ fs [FORALL_PROD]
+  \\ fs [padLen_DEC_eq,ADD1]
+QED
+
+val _ = fromChars_unsafe_ind |> update_precondition;
+
+val result = translate fromString_unsafe_def;
+
+val fromstring_unsafe_side_def = definition"fromstring_unsafe_side_def";
+val fromchars_unsafe_side_def = theorem"fromchars_unsafe_side_def";
+val fromchars_range_unsafe_side_def = fetch "-" "fromchars_range_unsafe_side_def";
+
+Theorem fromchars_unsafe_side_thm[local]:
+   ∀n s. n ≤ strlen s ⇒ fromchars_unsafe_side n s
+Proof
+  completeInduct_on`n` \\ rw[]
+  \\ rw[Once fromchars_unsafe_side_def,fromchars_range_unsafe_side_def,fromchars_range_unsafe_tail_side_def]
+QED
+
+Theorem fromString_unsafe_side[local]:
+  ∀x. fromstring_unsafe_side x = T
+Proof
+  Cases
+  \\ rw[fromstring_unsafe_side_def]
+  \\ Cases_on`s` \\ fs[mlstringTheory.substring_def]
+  \\ simp_tac bool_ss [ONE,SEG_SUC_CONS,SEG_LENGTH_ID]
+  \\ match_mp_tac fromchars_unsafe_side_thm
+  \\ rw[]
+QED
+
+val _ = update_precondition fromString_unsafe_side;
+
+val res = translate blanks_def;
+val res = translate tokenize_def;
+
+val res = translate mk_lit_def;
+
+val res = translate parse_until_zero_aux_def;
+val res = translate parse_until_zero_def;
+
+val res = translate parse_until_zero_nn_aux_def;
+val res = translate parse_until_zero_nn_def;
+
+val res = translate is_int_def;
+val res = translate tokenize_fast_def;
+
+val res = translate starts_with_def;
+
+Theorem EqualityType_CNF_LIT_TYPE:
+  EqualityType (CNF_LIT_TYPE NUM)
+Proof
+  metis_tac(eq_lemmas())
+QED
+
+(*** Building the initial formula array ***)
+
+Quote add_cakeml:
+  fun fill_arr arr i ls =
+    case ls of [] => arr
+    | (v::vs) =>
+      fill_arr (Array.updateResize arr None i (Some v)) (i+1) vs
+End
+
+Theorem fill_arr_spec:
+  ∀ls lsv arrv arrls arrlsv i iv.
+  NUM i iv ∧
+  LIST_TYPE a ls lsv ∧
+  LIST_REL (OPTION_TYPE a) arrls arrlsv
+  ⇒
+  app (p:'ffi ffi_proj) ^(fetch_v"fill_arr"(get_ml_prog_state()))
+  [arrv; iv; lsv]
+  (ARRAY arrv arrlsv)
+  (POSTv resv.
+    SEP_EXISTS arrlsv'. ARRAY resv arrlsv' *
+    &LIST_REL (OPTION_TYPE a)
+      (FOLDL (λacc (i,v). update_resize acc NONE (SOME v) i)
+        arrls (enumerate i ls)) arrlsv')
+Proof
+  Induct>>rw[]>>
+  xcf "fill_arr" (get_ml_prog_state ())>>
+  fs[LIST_TYPE_def,miscTheory.enumerate_def]>>
+  xmatch
+  >- (xvar>>xsimpl)>>
+  rpt xlet_autop>>
+  xlet`POSTv resv.
+    SEP_EXISTS arrlsv'. ARRAY resv arrlsv' *
+    &LIST_REL (OPTION_TYPE a) (update_resize arrls NONE (SOME h) i) arrlsv'`
+  >- (
+    xapp_spec array_updateResize_spec>>
+    xsimpl>>
+    first_x_assum (irule_at Any)>>
+    rw[]>>
+    irule LIST_REL_update_resize>>
+    gvs[OPTION_TYPE_def])>>
+  xapp>>xsimpl
+QED
+
+Quote add_cakeml:
+  fun build_fml_arr n k ls =
+    fill_arr (Array.array n None) k ls
+End
+
+Theorem build_fml_arr_spec:
+  NUM n nv ∧
+  NUM k kv ∧
+  LIST_TYPE a ls lsv
+  ⇒
+  app (p:'ffi ffi_proj) ^(fetch_v"build_fml_arr"(get_ml_prog_state()))
+  [nv; kv; lsv]
+  emp
+  (POSTv resv.
+    SEP_EXISTS arrlsv. ARRAY resv arrlsv *
+    &LIST_REL (OPTION_TYPE a) (build_fml_list k ls n) arrlsv)
+Proof
+  rw[]>>
+  xcf "build_fml_arr" (get_ml_prog_state ())>>
+  xlet_autop>>
+  xlet_auto_spec (SOME array_alloc_spec)>>
+  xapp>>
+  xsimpl>>
+  first_x_assum (irule_at Any)>>
+  qexistsl_tac [`k`,`REPLICATE n NONE`]>>
+  simp[build_fml_list_def,LIST_REL_REPLICATE_same,OPTION_TYPE_def]
+QED
