examples/cnf/lrup/array/lrup_arrayFullProgScript.sml
@@ -1,0 +1,711 @@
+(*
+  This builds the cake_lrup proof checker
+*)
+Theory lrup_arrayFullProg
+Ancestors
+  misc UnsafeProof cnf ccnf ccnf_list ccnf_arrayProg ccnf_parseProg
+  syntax_helper lrup lrup_cnf lrup_list lrup_arrayProg
+  basis_ffi
+Libs
+  preamble basis
+
+val _ = translation_extends"lrup_arrayProg";
+
+val _ = translate parse_header_line_def;
+
+Theorem parse_header_line_side_thm[local]:
+  ∀x. parse_header_line_side x ⇔ T
+Proof
+  rw[definition"parse_header_line_side_def"]>>
+  intLib.ARITH_TAC
+QED
+
+val _ = parse_header_line_side_thm |> update_precondition;
+
+val _ = translate var_lit_def;
+val _ = translate parse_vclause_def;
+val _ = translate nocomment_line_def;
+
+val blanks_v_thm = fetch "ccnf_parseProg" "blanks_v_thm";
+val tokenize_v_thm = fetch "ccnf_parseProg" "tokenize_v_thm";
+
+val inputLineTokens_specialize =
+  inputLineTokens_spec_lines
+  |> Q.GEN `f` |> Q.SPEC`blanks`
+  |> Q.GEN `fv` |> Q.SPEC`blanks_v`
+  |> Q.GEN `g` |> Q.ISPEC`tokenize`
+  |> Q.GEN `gv` |> Q.ISPEC`tokenize_v`
+  |> Q.GEN `a` |> Q.ISPEC`SUM_TYPE STRING_TYPE INT`
+  |> SIMP_RULE std_ss [blanks_v_thm,tokenize_v_thm,blanks_def] ;
+
+Overload "VCFML_TYPE" = ``LIST_TYPE vcclause_TYPE``
+
+(* The DIMACS body is read one line at a time, tokenizing during input *)
+Quote add_cakeml:
+  fun parse_body_arr lno maxvar fd acc =
+  case TextIO.inputLineTokens #"\n" fd blanks tokenize of
+    None => Inr (List.rev acc)
+  | Some l =>
+    if nocomment_line l then
+      (case parse_vclause maxvar l of
+        None => Inl (format_dimacs_failure lno "failed to parse line")
+      | Some cl =>
+        parse_body_arr (lno+1) maxvar fd (cl::acc))
+    else parse_body_arr (lno+1) maxvar fd acc
+End
+
+Theorem parse_body_arr_spec:
+  !lines fd fdv fs maxvar maxvarv acc accv lno lnov.
+  NUM lno lnov ∧
+  NUM maxvar maxvarv ∧
+  VCFML_TYPE acc accv
+  ⇒
+  app (p : 'ffi ffi_proj)
+    ^(fetch_v "parse_body_arr" (get_ml_prog_state()))
+    [lnov; maxvarv; fdv; accv]
+    (STDIO fs * INSTREAM_LINES #"\n" fd fdv lines fs)
+    (POSTv v.
+      &
+      (∃err.
+      SUM_TYPE STRING_TYPE VCFML_TYPE
+        (case parse_body_gen parse_vclause maxvar
+          (FILTER nocomment_line (MAP toks lines)) acc of
+          NONE => INL err
+        | SOME x => INR x) v) *
+      SEP_EXISTS k lines'.
+         STDIO (forwardFD fs fd k) * INSTREAM_LINES #"\n" fd fdv lines' (forwardFD fs fd k))
+Proof
+  Induct>>
+  simp []>>
+  rpt strip_tac>>
+  xcf "parse_body_arr" (get_ml_prog_state ())
+  >- (
+    xlet ‘(POSTv v.
+            SEP_EXISTS k.
+                STDIO (forwardFD fs fd k) *
+                INSTREAM_LINES #"\n" fd fdv [] (forwardFD fs fd k) *
+                &OPTION_TYPE (LIST_TYPE (SUM_TYPE STRING_TYPE INT)) NONE v)’
+    >- (
+      xapp_spec inputLineTokens_specialize>>
+      qexistsl_tac [`emp`,‘[]’,‘fs’]>>
+      qexists_tac ‘fd’>>xsimpl>>fs [])>>
+    gvs[OPTION_TYPE_def]>>
+    xmatch>>
+    simp[parse_body_gen_def]>>
+    rpt xlet_autop>>
+    xcon>>xsimpl>>
+    simp[SUM_TYPE_def]>>
+    qexists_tac ‘k’>>xsimpl>>
+    qexists_tac `[]`>>xsimpl)>>
+  xlet ‘(POSTv v.
+          SEP_EXISTS k.
+              STDIO (forwardFD fs fd k) *
+              INSTREAM_LINES #"\n" fd fdv lines (forwardFD fs fd k) *
+              & OPTION_TYPE (LIST_TYPE (SUM_TYPE STRING_TYPE INT)) (SOME (toks h)) v)’
+  >- (
+    xapp_spec inputLineTokens_specialize>>
+    qexistsl_tac [`emp`,‘h::lines’,‘fs’]>>
+    qexists_tac ‘fd’>>xsimpl>>fs []>>
+    rw []>>qexists_tac ‘x’>>xsimpl>>
+    simp[toks_def])>>
+  gvs[OPTION_TYPE_def]>>
+  xmatch>>fs []>>
+  xlet_autop>>
+  reverse IF_CASES_TAC
+  >- (
+    xif >> asm_exists_tac>>xsimpl>>
+    xlet_autop>>
+    xapp>> xsimpl>>
+    rpt(first_x_assum (irule_at Any))>>
+    qexists_tac`forwardFD fs fd k`>>
+    qexists_tac`fd`>>xsimpl>>
+    rw[]>>
+    qexists_tac`k+x`>>
+    simp[GSYM fsFFIPropsTheory.forwardFD_o]>>
+    qexists_tac`x'`>>xsimpl>>
+    metis_tac[])>>
+  xif>> asm_exists_tac>>simp[]>>
+  xlet_autop>>
+  simp[parse_body_gen_def]>>
+  Cases_on`parse_vclause maxvar (toks h)`>>
+  fs[OPTION_TYPE_def]
+  >- (
+    xmatch>>
+    xlet_autop>>
+    xcon>>
+    xsimpl>>
+    qexists_tac`k`>> qexists_tac`lines`>>xsimpl>>
+    simp[SUM_TYPE_def]>>
+    metis_tac[])>>
+  rename1`parse_vclause maxvar (toks h) = SOME cl`>>
+  xmatch>>
+  xlet_autop>>
+  xlet_autop>>
+  xapp>>
+  xsimpl>>
+  rpt(first_x_assum (irule_at Any))>>
+  qexistsl_tac [`forwardFD fs fd k`,`fd`]>>
+  xsimpl>>
+  simp[LIST_TYPE_def,forwardFD_o]>>rw[]>>
+  qexists_tac`cl::acc`>>
+  simp[LIST_TYPE_def]>>
+  rw[]>>
+  qexistsl_tac [`k+x`,`x'`]>>
+  xsimpl>>
+  metis_tac[]
+QED
+
+Quote add_cakeml:
+  fun parse_vcnf_toks_arr lno fd =
+  case TextIO.inputLineTokens #"\n" fd blanks tokenize of
+    None => Inl (format_dimacs_failure lno "failed to find header")
+  | Some l =>
+    if nocomment_line l then
+      (case parse_header_line l of
+        None => Inl (format_dimacs_failure lno "failed to parse header")
+      | Some res => case res of (vars,ncl) =>
+        (case parse_body_arr lno vars fd [] of
+          Inl fail => Inl fail
+        | Inr acc =>
+          if List.length acc = ncl then
+            Inr (vars,(ncl,acc))
+          else
+            Inl (format_dimacs_failure lno "incorrect number of clauses")))
+    else parse_vcnf_toks_arr (lno+1) fd
+End
+
+Theorem parse_vcnf_toks_arr_spec:
+  !lines fd fdv fs lno lnov.
+  NUM lno lnov
+  ⇒
+  app (p : 'ffi ffi_proj)
+    ^(fetch_v "parse_vcnf_toks_arr" (get_ml_prog_state()))
+    [lnov; fdv]
+    (STDIO fs * INSTREAM_LINES #"\n" fd fdv lines fs)
+    (POSTv v.
+      & (∃err. SUM_TYPE STRING_TYPE
+        (PAIR_TYPE NUM (PAIR_TYPE NUM VCFML_TYPE))
+      (case parse_vcnf_toks (MAP toks lines) of
+        NONE => INL err
+      | SOME x => INR x) v) *
+      SEP_EXISTS k lines'.
+         STDIO (forwardFD fs fd k) * INSTREAM_LINES #"\n" fd fdv lines' (forwardFD fs fd k))
+Proof
+  Induct>>
+  simp []>>
+  rpt strip_tac>>
+  xcf "parse_vcnf_toks_arr" (get_ml_prog_state ())
+  >- (
+    xlet ‘(POSTv v.
+            SEP_EXISTS k.
+                STDIO (forwardFD fs fd k) *
+                INSTREAM_LINES #"\n" fd fdv [] (forwardFD fs fd k) *
+                &OPTION_TYPE (LIST_TYPE (SUM_TYPE STRING_TYPE INT)) NONE v)’
+    >- (
+      xapp_spec inputLineTokens_specialize>>
+      qexistsl_tac [`emp`,‘[]’,‘fs’]>>
+      qexists_tac ‘fd’>>xsimpl>>fs [])>>
+    gvs [OPTION_TYPE_def]>>
+    xmatch>>fs []>>
+    simp[parse_vcnf_toks_def,parse_dimacs_toks_gen_def]>>
+    xlet_autop>>
+    xcon>>xsimpl>>
+    simp[SUM_TYPE_def]>>
+    qexists_tac ‘k’>>xsimpl>>
+    qexists_tac `[]`>>xsimpl>>
+    metis_tac[])>>
+  xlet ‘(POSTv v.
+          SEP_EXISTS k.
+              STDIO (forwardFD fs fd k) *
+              INSTREAM_LINES #"\n" fd fdv lines (forwardFD fs fd k) *
+              & OPTION_TYPE (LIST_TYPE (SUM_TYPE STRING_TYPE INT)) (SOME (toks h)) v)’
+  >- (
+    xapp_spec inputLineTokens_specialize>>
+    qexistsl_tac [`emp`,‘h::lines’,‘fs’]>>
+    qexists_tac ‘fd’>>xsimpl>>fs []>>
+    rw []>>qexists_tac ‘x’>>xsimpl>>
+    simp[toks_def])>>
+  gvs [OPTION_TYPE_def]>>
+  xmatch>>fs []>>
+  xlet_autop>>
+  simp[parse_vcnf_toks_def,parse_dimacs_toks_gen_def]>>
+  reverse IF_CASES_TAC
+  >- (
+    xif >> asm_exists_tac>>xsimpl>>
+    xlet_autop>>
+    xapp>> xsimpl>>
+    asm_exists_tac>> simp[]>>
+    qexists_tac`emp`>>xsimpl>>
+    qexists_tac`forwardFD fs fd k`>>
+    qexists_tac`fd`>>xsimpl>>
+    rw[]>>
+    fs[parse_vcnf_toks_def,parse_dimacs_toks_gen_def]>>
+    qexists_tac`k+x`>>
+    simp[GSYM fsFFIPropsTheory.forwardFD_o]>>
+    qexists_tac`x'`>>xsimpl>>
+    metis_tac[])>>
+  xif>> asm_exists_tac>>simp[]>>
+  xlet_autop>>
+  Cases_on`parse_header_line (toks h)`>>fs[OPTION_TYPE_def]
+  >- (
+    xmatch>>
+    xlet_autop>>
+    xcon>>
+    xsimpl>>
+    qexists_tac`k`>> qexists_tac`lines`>>xsimpl>>
+    simp[SUM_TYPE_def]>>
+    metis_tac[])>>
+  xmatch>>
+  rename1`parse_header_line (toks h) = SOME hdr`>>
+  PairCases_on`hdr`>>fs[PAIR_TYPE_def]>>
+  xmatch>>
+  xlet_autop>>
+  xlet `(POSTv v.
+      & (∃err. SUM_TYPE STRING_TYPE VCFML_TYPE
+      (case parse_body_gen parse_vclause hdr0
+        (FILTER nocomment_line (MAP toks lines)) [] of
+        NONE => INL err
+      | SOME x => INR x) v) *
+      SEP_EXISTS k lines'.
+         STDIO (forwardFD fs fd k) * INSTREAM_LINES #"\n" fd fdv lines' (forwardFD fs fd k))`
+  >- (
+    xapp>>xsimpl>>
+    qexistsl_tac [`emp`,`hdr0`,`lines`,`forwardFD fs fd k`,`fd`,`[]`,
+      `lno`]>>
+    xsimpl>>
+    simp[LIST_TYPE_def]>>
+    rw[]>>
+    qexists_tac`k+x`>>
+    simp[GSYM fsFFIPropsTheory.forwardFD_o]>>
+    qexists_tac`x'`>>xsimpl>>
+    metis_tac[])>>
+  pop_assum mp_tac>> TOP_CASE_TAC>>fs[OPTION_TYPE_def]
+  >- (
+    rw[]>>fs[SUM_TYPE_def]>>
+    xmatch>>
+    xcon>>
+    xsimpl>>
+    qexists_tac`k`>>qexists_tac`lines'`>>xsimpl>>
+    metis_tac[])>>
+  strip_tac>>fs[SUM_TYPE_def]>>
+  xmatch>>
+  drule LENGTH_parse_body_gen>>
+  strip_tac>>gvs[]>>
+  rpt xlet_autop>>
+  rw[]>>xif
+  >- (
+    asm_exists_tac>>simp[]>>
+    rpt xlet_autop>>
+    xcon>>xsimpl>>
+    simp[SUM_TYPE_def,PAIR_TYPE_def]>>
+    qexists_tac`k`>>qexists_tac`lines'`>>xsimpl)>>
+  asm_exists_tac>>simp[]>>
+  xlet_autop>>
+  xcon>>
+  xsimpl>>
+  qexistsl_tac [`k`,`lines'`]>>
+  simp[SUM_TYPE_def]>>
+  xsimpl>>
+  metis_tac[]
+QED
+
+(* parse_vcnf_toks with simple wrapper *)
+Quote add_cakeml:
+  fun parse_full fname =
+  let
+    val fd = TextIO.openIn fname
+    val res = parse_vcnf_toks_arr 0 fd
+    val close = TextIO.closeIn fd;
+  in
+    res
+  end
+  handle TextIO.BadFileName => Inl (notfound_string fname)
+End
+
+Theorem parse_full_spec:
+  STRING_TYPE f fv ∧
+  validArg f ∧
+  hasFreeFD fs
+  ⇒
+  app (p:'ffi ffi_proj) ^(fetch_v"parse_full"(get_ml_prog_state()))
+    [fv]
+    (STDIO fs)
+    (POSTv v.
+    & (∃err. (SUM_TYPE STRING_TYPE (PAIR_TYPE NUM (PAIR_TYPE NUM VCFML_TYPE))
+    (if inFS_fname fs f then
+    (case parse_vcnf_toks (MAP toks (all_lines_file fs f)) of
+      NONE => INL err
+    | SOME x => INR x)
+    else INL err) v)) * STDIO fs)
+Proof
+  rw[]>>
+  xcf"parse_full"(get_ml_prog_state()) >>
+  fs[validArg_def]>>
+  reverse (Cases_on `STD_streams fs`)
+  >- (fs [TextIOProofTheory.STDIO_def]>>xpull) >>
+  reverse (Cases_on`consistentFS fs`)
+  >- (fs [STDIO_def,IOFS_def,wfFS_def,consistentFS_def]>>xpull>>metis_tac[]) >>
+  reverse (Cases_on `inFS_fname fs f`) >> simp[]
+  >- (
+    xhandle`POSTe ev.
+      &BadFileName_exn ev *
+      &(~inFS_fname fs f) *
+      STDIO fs`
+    >-
+      (xlet_auto_spec (SOME openIn_STDIO_spec)>>xsimpl)
+    >>
+      fs[BadFileName_exn_def]>>
+      xcases>>rw[]>>
+      xlet_auto>>xsimpl>>
+      xcon>>xsimpl>>
+      simp[SUM_TYPE_def]>>metis_tac[])>>
+  qmatch_goalsub_abbrev_tac`$POSTv Qval`>>
+  xhandle`$POSTv Qval`>>xsimpl>>
+  qunabbrev_tac`Qval`>>
+  xlet_auto_spec (SOME (openIn_spec_lines |> Q.GEN `c0` |> Q.SPEC `#"\n"`))>>xsimpl>>
+  qmatch_goalsub_abbrev_tac`STDIO fss`>>
+  qmatch_goalsub_abbrev_tac`INSTREAM_LINES _ fdd fddv lines fss`>>
+  xlet`(POSTv v.
+      & (∃err. SUM_TYPE STRING_TYPE (PAIR_TYPE NUM (PAIR_TYPE NUM VCFML_TYPE))
+      (case parse_vcnf_toks (MAP toks lines) of
+        NONE => INL err
+      | SOME x => INR x) v) *
+      SEP_EXISTS k lines'.
+         STDIO (forwardFD fss fdd k) * INSTREAM_LINES #"\n" fdd fddv lines' (forwardFD fss fdd k))`
+  >- (
+    xapp>>xsimpl>>
+    qexists_tac`emp`>>qexists_tac`lines`>>
+    qexists_tac`fss`>>qexists_tac`fdd`>>xsimpl>>
+    rw[]>>
+    qexists_tac`x`>>qexists_tac`x'`>>xsimpl>>
+    metis_tac[])>>
+  xlet `POSTv v. STDIO fs`
+  >- (
+    xapp_spec closeIn_spec_lines >>
+    qexistsl_tac [`emp`,`lines'`,`forwardFD fss fdd k`,`fdd`,`#"\n"`]>>
+    conj_tac >-
+     (unabbrev_all_tac>>
+      imp_res_tac fsFFIPropsTheory.nextFD_ltX>>fs []>>
+      imp_res_tac fsFFIPropsTheory.STD_streams_nextFD>>fs []) >>
+    xsimpl>>
+    `validFileFD fdd (forwardFD fss fdd k).infds` by
+      (unabbrev_all_tac>> simp[validFileFD_forwardFD]>>
+       imp_res_tac fsFFIPropsTheory.nextFD_ltX>>fs []>>
+       match_mp_tac validFileFD_nextFD>>fs []) >>
+    xsimpl >> rw [] >>
+    imp_res_tac (DECIDE ``n<m:num ==> n <= m``) >>
+    imp_res_tac fsFFIPropsTheory.nextFD_leX>>fs [] >>
+    drule fsFFIPropsTheory.openFileFS_ADELKEY_nextFD >>
+    fs [Abbr`fss`]>>xsimpl)>>
+  xvar>>
+  xsimpl>>
+  metis_tac[]
+QED
+
+val usage_string = ‘
+
+Usage:  cake_lrup <CNF formula file> <optional: compressed LRUP proof file>
+
+Run LRUP unsatisfiability proof checking (if proof is given)
+
+’
+
+fun drop_until p [] = []
+  | drop_until p (x::xs) = if p x then x::xs else drop_until p xs;
+
+val usage_string_tm =
+  usage_string |> hd |> (fn QUOTE s => s) |> explode
+  |> drop_until (fn c => c = #"\n") |> tl |> implode
+  |> stringSyntax.fromMLstring;
+
+Definition usage_string_def:
+  usage_string = strlit ^usage_string_tm
+End
+
+val r = translate usage_string_def;
+
+(*
+  Checker takes up to 2 arguments:
+  2 args (CNF file, proof file):
+    parse CNF, run proof, report UNSAT (or error)
+
+  The RUP assignment array is indexed by the ORIGINAL variable, so mv+1
+  slots suffice for the initial formula (every literal satisfies
+  var_lit l ≤ mv by check_maxvar). It grows on demand thereafter.
+*)
+Quote add_cakeml:
+  fun check_unsat_2 f1 f2 =
+  case parse_full f1 of
+    Inl err => TextIO.output TextIO.stdErr err
+  | Inr (mv,(ncl,vcfml)) =>
+    (case check_unsat' vcfml f2 (mv+1) (2*ncl) of
+      Inl err => TextIO.output TextIO.stdErr err
+    | Inr b =>
+      if b then
+        TextIO.print "s VERIFIED UNSAT\n"
+      else
+        TextIO.output TextIO.stdErr "c empty clause not derived at end of proof\n")
+End
+
+val _ = translate print_lit_def;
+val _ = translate print_lits_def;
+val _ = translate max_list_def;
+val _ = translate max_cnf_def;
+val _ = translate print_header_line_def;
+val _ = translate print_cnf_def;
+val _ = translate unconv_cfml_def;
+
+Quote add_cakeml:
+  fun check_unsat_1 f1 =
+  case parse_full f1 of
+    Inl err => TextIO.output TextIO.stdErr err
+  | Inr (mv,(ncl,vcfml)) => TextIO.print_list (print_cnf (unconv_cfml vcfml))
+End
+
+(* The formula a run of the checker is about: the contents of the input
+  file, when it exists and parses *)
+Definition get_cnf_def:
+  get_cnf fs f =
+  if inFS_fname fs f
+  then parse_cnf (all_lines_file fs f)
+  else NONE
+End
+
+Definition check_unsat_1_sem_def:
+  check_unsat_1_sem fs f1 out ⇔
+  case get_cnf fs f1 of
+    SOME fml => out = concat (print_cnf fml)
+  | NONE => out = «»
+End
+
+(* Every failure path prints nothing on stdout and reports err on stderr.
+  out_tac supplies the empty stdout witness on the paths where the output
+  predicate does not already pin it. *)
+fun err_tac out_tac =
+  xapp_spec output_stderr_spec>>xsimpl>>
+  asm_exists_tac>>xsimpl>>
+  qexists_tac`emp`>>qexists_tac`fs`>>xsimpl>>
+  rw[]>>out_tac>>
+  qexists_tac`err`>>
+  fs[STD_streams_add_stderr,STD_streams_stdout,add_stdo_nil]>>
+  xsimpl;
+
+val no_out = qexists_tac`«»`;
+
+Theorem check_unsat_1_spec:
+  STRING_TYPE f1 f1v ∧
+  validArg f1 ∧
+  hasFreeFD fs
+  ⇒
+  app (p:'ffi ffi_proj) ^(fetch_v"check_unsat_1"(get_ml_prog_state()))
+    [f1v]
+    (STDIO fs)
+    (POSTv uv. &UNIT_TYPE () uv *
+    SEP_EXISTS out err.
+      STDIO (add_stdout (add_stderr fs err) out) *
+      &(check_unsat_1_sem fs f1 out))
+Proof
+  rw[]>>
+  xcf "check_unsat_1" (get_ml_prog_state ())>>
+  reverse (Cases_on `STD_streams fs`)
+  >- (fs [TextIOProofTheory.STDIO_def]>>xpull)>>
+  xlet_autop>>
+  simp[check_unsat_1_sem_def,get_cnf_def,parse_cnf_def]>>
+  reverse (Cases_on`inFS_fname fs f1`)>>fs[SUM_TYPE_def,parse_vcnf_toks]
+  >- (xmatch>>err_tac all_tac)>>
+  Cases_on`parse_cnf_toks (MAP toks (all_lines_file fs f1))`>>
+  fs[SUM_TYPE_def]
+  >- (xmatch>>err_tac all_tac)>>
+  PairCases_on`x`>>
+  gvs[PAIR_TYPE_def]>>
+  rename1`parse_cnf_toks _ = SOME (mv,ncl,fml)`>>
+  xmatch>>
+  xlet_autop>>
+  `unconv_cfml (conv_cfml fml) = fml` by
+    metis_tac[unconv_cfml_conv_cfml,parse_cnf_toks_nz_lit]>>
+  gvs[]>>
+  xlet_autop>>
+  xapp_spec print_list_spec>>xsimpl>>
+  asm_exists_tac>>xsimpl>>
+  qexists_tac`emp`>>qexists_tac`fs`>>xsimpl>>
+  rw[]>>
+  qexists_tac`«»`>>
+  simp[STD_streams_stderr,add_stdo_nil]>>
+  xsimpl
+QED
+
+Quote add_cakeml:
+  fun check_unsat u =
+  case CommandLine.arguments () of
+    [f1] => check_unsat_1 f1
+  | [f1,f2] => check_unsat_2 f1 f2
+  | _ => TextIO.output TextIO.stdErr usage_string
+End
+
+Definition check_unsat_2_sem_def:
+  check_unsat_2_sem fs f1 out ⇔
+  (out ≠ «» ⇒
+    out = «s VERIFIED UNSAT\n» ∧
+    ∃fml. get_cnf fs f1 = SOME fml ∧ sols fml = {})
+End
+
+Theorem check_unsat_2_spec:
+  STRING_TYPE f1 f1v ∧ validArg f1 ∧
+  STRING_TYPE f2 f2v ∧ validArg f2 ∧
+  hasFreeFD fs
+  ⇒
+  app (p:'ffi ffi_proj) ^(fetch_v"check_unsat_2"(get_ml_prog_state()))
+    [f1v; f2v]
+    (STDIO fs)
+    (POSTv uv. &UNIT_TYPE () uv *
+    SEP_EXISTS out err.
+      STDIO (add_stdout (add_stderr fs err) out) *
+      &(check_unsat_2_sem fs f1 out))
+Proof
+  rw[]>>
+  xcf "check_unsat_2" (get_ml_prog_state ())>>
+  reverse (Cases_on `STD_streams fs`)
+  >- (fs [TextIOProofTheory.STDIO_def]>>xpull)>>
+  xlet_autop>>
+  simp[check_unsat_2_sem_def,get_cnf_def,parse_cnf_def]>>
+  reverse (Cases_on`inFS_fname fs f1`)>>fs[SUM_TYPE_def,parse_vcnf_toks]
+  >- (xmatch>>err_tac all_tac)>>
+  Cases_on`parse_cnf_toks (MAP toks (all_lines_file fs f1))`>>
+  fs[SUM_TYPE_def]
+  >- (xmatch>>err_tac all_tac)>>
+  qmatch_asmsub_rename_tac`parse_cnf_toks _ = SOME res`>>
+  PairCases_on`res`>>
+  gvs[SUM_TYPE_def,PAIR_TYPE_def]>>
+  rename1`parse_cnf_toks _ = SOME (mv,ncl,cfml)`>>
+  xmatch>>
+  rpt xlet_autop>>
+  xlet`POSTv v.
+    STDIO fs *
+    SEP_EXISTS res.
+      &(SUM_TYPE STRING_TYPE BOOL res v ∧
+        (res = INR T ⇒ sols cfml = {}))`
+  >- (
+    xapp>>
+    rw[]
+    >- metis_tac[parse_cnf_toks_nz_lit]
+    >- (
+      qexists_tac`f2`>>
+      fs[FILENAME_def,validArg_def])
+    >- (
+      qexists_tac`mv+1`>>simp[]>>
+      drule parse_cnf_toks_bound>>
+      rw[EVERY_MEM]>>res_tac>>simp[])>>
+    qexists_tac`2*ncl`>>simp[])>>
+  namedCases_on`res` ["err","b"]>>fs[SUM_TYPE_def]
+  >- (
+    xmatch>>err_tac no_out)>>
+  xmatch>>
+  xif
+  >- (
+    xapp_spec print_spec>>xsimpl>>
+    qexists_tac`emp`>>qexists_tac`fs`>>xsimpl>>
+    rw[]>>
+    qexistsl_tac [`«s VERIFIED UNSAT\n»`,`«»`]>>
+    simp[STD_streams_stderr,add_stdo_nil]>>
+    xsimpl)>>
+  xapp_spec output_stderr_spec>>xsimpl>>
+  qexists_tac`emp`>>qexists_tac`fs`>>xsimpl>>
+  rw[]>>
+  qexistsl_tac [`«»`,`«c empty clause not derived at end of proof\n»`]>>
+  fs[STD_streams_add_stderr,STD_streams_stdout,add_stdo_nil]>>
+  xsimpl
+QED
+
+Definition check_unsat_sem_def:
+  check_unsat_sem fs cl out ⇔
+  if LENGTH cl = 2 then check_unsat_1_sem fs (EL 1 cl) out
+  else if LENGTH cl = 3 then check_unsat_2_sem fs (EL 1 cl) out
+  else out = «»
+End
+
+Theorem STDIO_refl:
+  STDIO A ==>>
+  STDIO A * GC
+Proof
+  xsimpl
+QED
+
+Theorem check_unsat_spec:
+   hasFreeFD fs
+   ⇒
+   app (p:'ffi ffi_proj) ^(fetch_v"check_unsat"(get_ml_prog_state()))
+     [Conv NONE []]
+     (COMMANDLINE cl * STDIO fs)
+     (POSTv uv. &UNIT_TYPE () uv *
+     COMMANDLINE cl *
+     SEP_EXISTS out err.
+       STDIO (add_stdout (add_stderr fs err) out) *
+       &(check_unsat_sem fs cl out))
+Proof
+  rw[check_unsat_sem_def]>>
+  xcf"check_unsat"(get_ml_prog_state())>>
+  reverse (Cases_on `STD_streams fs`)
+  >- (fs [TextIOProofTheory.STDIO_def]>>xpull)>>
+  reverse(Cases_on`wfcl cl`) >- (fs[COMMANDLINE_def]>>xpull)>>
+  rpt xlet_autop >>
+  Cases_on `cl` >- fs[wfcl_def] >>
+  Cases_on`t`>>fs[LIST_TYPE_def]
+  >- (
+    xmatch>>
+    xapp_spec output_stderr_spec>>xsimpl>>
+    rename1`COMMANDLINE cl`>>
+    qexists_tac`COMMANDLINE cl`>>xsimpl>>
+    qexists_tac`usage_string`>>
+    simp[theorem "usage_string_v_thm"]>>
+    qexists_tac`fs`>>xsimpl>>
+    rw[]>>
+    fs[STD_streams_add_stderr,STD_streams_stdout,add_stdo_nil]>>
+    metis_tac[STDIO_refl])>>
+  Cases_on`t'`>>fs[LIST_TYPE_def]
+  >- (
+    xmatch>>
+    xapp>>rw[]>>
+    rpt(first_x_assum (irule_at Any)>>xsimpl)>>
+    fs[wfcl_def]>>
+    rw[]>>metis_tac[STDIO_refl])>>
+  Cases_on`t`>>fs[LIST_TYPE_def]
+  >- (
+    xmatch>>
+    xapp>>rw[]>>
+    rpt(first_x_assum (irule_at Any)>>xsimpl)>>
+    fs[wfcl_def]>>
+    rw[]>>metis_tac[STDIO_refl])>>
+  xmatch>>
+  xapp_spec output_stderr_spec>>xsimpl>>
+  rename1`COMMANDLINE cl`>>
+  qexists_tac`COMMANDLINE cl`>>xsimpl>>
+  qexists_tac`usage_string`>>
+  simp[theorem "usage_string_v_thm"]>>
+  qexists_tac`fs`>>xsimpl>>
+  rw[]>>
+  fs[STD_streams_add_stderr,STD_streams_stdout,add_stdo_nil]>>
+  metis_tac[STDIO_refl]
+QED
+
+Theorem check_unsat_whole_prog_spec2:
+   hasFreeFD fs ⇒
+   whole_prog_spec2 check_unsat_v cl fs NONE
+     (λfs'. ∃out err.
+        fs' = add_stdout (add_stderr fs err) out ∧
+        check_unsat_sem fs cl out)
+Proof
+  rw[basis_ffiTheory.whole_prog_spec2_def]>>
+  match_mp_tac (MP_CANON (DISCH_ALL (MATCH_MP app_wgframe (UNDISCH check_unsat_spec))))>>
+  xsimpl>>
+  rw[PULL_EXISTS]>>
+  qexists_tac`add_stdout (add_stderr fs x') x`>>
+  xsimpl>>
+  qexistsl_tac [`x`,`x'`]>>
+  xsimpl>>
+  simp[GSYM add_stdo_with_numchars,with_same_numchars]
+QED
+
+Theorem check_unsat_semantics =
+  prove_sem_thm "check_unsat"
+                "check_unsat_prog"
+                check_unsat_whole_prog_spec2;
