examples/cnf/lrup/array/lrup_arrayProgScript.sml
@@ -1,0 +1,633 @@
+(*
+  This refines lrup_list to use arrays
+*)
+Theory lrup_arrayProg
+Ancestors
+  misc mllist UnsafeProof ccnf_arrayProg ccnf_parseProg cnf ccnf ccnf_list
+  syntax_helper lrup_cnf lrup lrup_list
+  mlint mlvector
+Libs
+  preamble basis
+
+val _ = hide_environments true;
+
+val _ = translation_extends "ccnf_parseProg";
+
+val _ = register_type``:lrup``;
+
+Quote add_cakeml:
+  fun check_lrup_arr lno lrup fml carr b =
+  case lrup of
+    Delvb s =>
+      (delete_ids_vb_arr fml s 1 (String.size s); (fml, carr, b))
+  | Lrupvb n c s =>
+      (case is_rup_vb_arr lno fml carr b c s of (carr,b) =>
+        (Array.updateResize fml None n (Some c), carr, b))
+End
+
+val LRUP_LRUP_TYPE_def = fetch "-" "LRUP_LRUP_TYPE_def";
+
+Theorem check_lrup_arr_spec:
+  NUM lno lnov ∧
+  LRUP_LRUP_TYPE lrup lrupv ∧
+  LIST_REL (OPTION_TYPE vcclause_TYPE) fmlls fmllsv ∧
+  WORD8 b bv ∧
+  bnd_fml fmlls (LENGTH Clist)
+  ⇒
+  app (p : 'ffi ffi_proj)
+    ^(fetch_v "check_lrup_arr" (get_ml_prog_state()))
+    [lnov; lrupv; fmlv; Carrv; bv]
+    (ARRAY fmlv fmllsv * W8ARRAY Carrv Clist)
+    (POSTve
+      (λv.
+        SEP_EXISTS v1 v2 v3.
+          &(v = Conv NONE [v1; v2; v3]) *
+          (SEP_EXISTS fmllsv' clist'.
+            ARRAY v1 fmllsv' *
+            W8ARRAY v2 clist' *
+            &(
+            case check_lrup_list lrup fmlls Clist b of
+              NONE => F
+            | SOME (fmlls', Clist', b') =>
+                bnd_fml fmlls' (LENGTH Clist') ∧
+                LIST_REL (OPTION_TYPE vcclause_TYPE) fmlls' fmllsv' ∧
+                WORD8 b' v3 ∧
+                Clist' = clist'
+            ))
+      )
+      (λe. ARRAY fmlv fmllsv *
+        &(Fail_exn e ∧
+        check_lrup_list lrup fmlls Clist b = NONE)))
+Proof
+  rw[check_lrup_list_def]>>
+  xcf "check_lrup_arr" (get_ml_prog_state ())>>
+  Cases_on`lrup`>>fs[LRUP_LRUP_TYPE_def]
+  >- (
+    (* Delvb *)
+    xmatch>>
+    rpt xlet_autop>>
+    xcon>>xsimpl>>
+    metis_tac[bnd_fml_delete_ids_vb_list])>>
+  (* Lrupvb *)
+  xmatch>>
+  xlet `
+    POSTve
+      (λres.
+           (SEP_EXISTS b' Carrv' Clist'.
+              W8ARRAY Carrv' Clist' *
+              &(PAIR_TYPE $= WORD8 (Carrv',b') res ∧
+               is_rup_vb_list fmlls Clist b v m = (T,Clist',b'))) *
+           ARRAY fmlv fmllsv)
+      (λe.
+          ARRAY fmlv fmllsv *
+          &(Fail_exn e ∧ ¬FST (is_rup_vb_list fmlls Clist b v m)))`
+  >- (
+    xapp>>xsimpl>>
+    rpt(first_x_assum (irule_at Any))>>
+    simp[PAIR_TYPE_def]>>rw[]>>
+    xsimpl)
+  >- (
+    xsimpl>>rw[]>>
+    every_case_tac>>gvs[])>>
+  gvs[PAIR_TYPE_def]>>
+  xmatch>>
+  rpt xlet_autop>>
+  xcon>>xsimpl>>
+  gvs[]>>
+  CONJ_TAC >- (
+    irule bnd_fml_update_resize>>
+    metis_tac[bnd_fml_is_rup_vb_list])>>
+  irule LIST_REL_update_resize>>
+  simp[OPTION_TYPE_def]
+QED
+
+(*** Reading and checking a proof file, one record at a time ***)
+
+Theorem SEP_IMP_REFL_gc[local]:
+  p ==>> p * GC
+Proof
+  xsimpl
+QED
+
+(* Closes a separation-logic entailment whose two sides differ only by
+  frame association and GC slack *)
+val sep_triv = metis_tac[SEP_IMP_REFL_gc,SEP_IMP_REFL,STAR_ASSOC,STAR_COMM];
+
+(* Records are terminated by a zero byte *)
+Definition nulc_def:
+  nulc = CHR 0
+End
+
+val nulc_v_thm = translate nulc_def;
+
+val res = translate vb_ilit_def;
+val res = translate parse_vb_ilits_def;
+
+Theorem parse_vb_ilits_side[local]:
+  ∀s i len acc.
+  len ≤ strlen s ⇒ parse_vb_ilits_side s i len acc
+Proof
+  ho_match_mp_tac parse_vb_ilits_ind>>
+  rw[]>>
+  simp[Once (fetch "-" "parse_vb_ilits_side_def")]>>
+  simp[fetch "ccnf_arrayProg" "parse_vb_num_side_def",parse_vb_num_aux_side]
+QED
+
+val _ = parse_vb_ilits_side |> update_precondition;
+
+val res = translate parse_lrup_chunk_def;
+
+Theorem parse_lrup_chunk_side[local]:
+  ∀s. parse_lrup_chunk_side s
+Proof
+  rw[fetch "-" "parse_lrup_chunk_side_def"]>>
+  simp[parse_vb_ilits_side,fetch "ccnf_arrayProg" "parse_vb_num_side_def",
+    parse_vb_num_aux_side]
+QED
+
+val _ = parse_lrup_chunk_side |> update_precondition;
+
+Quote add_cakeml:
+  fun parse_lrup_one_arr lno fd =
+  case TextIO.inputLineWith nulc fd of
+    None => None
+  | Some l =>
+    (case parse_lrup_chunk l of
+      None =>
+        raise Fail (format_failure lno "failed to parse compressed LRUP record")
+    | Some (Inl step) => Some step
+    | Some (Inr idc) =>
+      case idc of (id,c) =>
+        (case TextIO.inputLineWith nulc fd of
+          None =>
+            raise Fail (format_failure lno "missing RUP hints")
+        | Some h => Some (Lrupvb id c h)))
+End
+
+Theorem parse_lrup_one_arr_spec:
+  NUM lno lnov
+  ⇒
+  app (p : 'ffi ffi_proj)
+    ^(fetch_v "parse_lrup_one_arr" (get_ml_prog_state()))
+    [lnov; fdv]
+    (STDIO fs * INSTREAM_LINES nulc fd fdv lines fs)
+    (POSTve
+      (λv.
+        SEP_EXISTS k lines'.
+          STDIO (forwardFD fs fd k) *
+          INSTREAM_LINES nulc fd fdv lines' (forwardFD fs fd k) *
+          &(parse_lrup_one lines ≠ NONE ∧
+            OPTION_TYPE LRUP_LRUP_TYPE
+              (OPTION_MAP FST (THE (parse_lrup_one lines))) v ∧
+            (case THE (parse_lrup_one lines) of
+              NONE => lines' = []
+            | SOME res => lines' = SND res)))
+      (λe.
+        SEP_EXISTS k lines'.
+          STDIO (forwardFD fs fd k) *
+          INSTREAM_LINES nulc fd fdv lines' (forwardFD fs fd k) *
+          &(Fail_exn e ∧ parse_lrup_one lines = NONE)))
+Proof
+  rw[]>>
+  xcf "parse_lrup_one_arr" (get_ml_prog_state ())>>
+  xlet `POSTv v.
+    SEP_EXISTS k.
+      STDIO (forwardFD fs fd k) *
+      INSTREAM_LINES nulc fd fdv (TL lines) (forwardFD fs fd k) *
+      &OPTION_TYPE STRING_TYPE (oHD lines) v`
+  >- (
+    xapp>>
+    simp[nulc_v_thm])>>
+  simp[parse_lrup_one_def]>>
+  Cases_on`lines`>>fs[OPTION_TYPE_def]>>xmatch
+  >- (
+    xcon>>xsimpl>>
+    sep_triv)>>
+  xlet_autop>>
+  Cases_on`parse_lrup_chunk h`>>fs[OPTION_TYPE_def]
+  >- (
+    xmatch>>
+    rpt xlet_autop>>
+    xraise>>xsimpl>>
+    gvs[Fail_exn_def]>>
+    first_x_assum (irule_at Any)>>
+    sep_triv)>>
+  rename1`parse_lrup_chunk h = SOME res`>>
+  Cases_on`res`>>fs[SUM_TYPE_def]>>xmatch
+  >- (
+    xcon>>xsimpl>>
+    simp[OPTION_TYPE_def]>>
+    sep_triv)>>
+  rename1`INSTREAM_LINES nulc fd fdv lines`>>
+  rename1`parse_lrup_chunk h = SOME (INR idc)`>>
+  Cases_on`idc`>>gvs[PAIR_TYPE_def]>>
+  xmatch>>
+  xlet `POSTv v.
+    SEP_EXISTS k.
+      STDIO (forwardFD fs fd k) *
+      INSTREAM_LINES nulc fd fdv (TL lines) (forwardFD fs fd k) *
+      &OPTION_TYPE STRING_TYPE (oHD lines) v`
+  >- (
+    xapp>>
+    irule_at Any nulc_v_thm>>xsimpl>>
+    qexistsl_tac [`lines`,`forwardFD fs fd k`,`fd`]>>
+    xsimpl>>
+    simp[forwardFD_o]>>
+    sep_triv)>>
+  Cases_on`lines`>>fs[OPTION_TYPE_def]>>
+  xmatch
+  >- (
+    rpt xlet_autop>>
+    xraise>>xsimpl>>
+    gvs[Fail_exn_def]>>
+    first_x_assum (irule_at Any)>>
+    sep_triv)>>
+  xlet_autop>>
+  xcon>>xsimpl>>
+  simp[OPTION_TYPE_def,LRUP_LRUP_TYPE_def]>>
+  qexists_tac`k`>>
+  xsimpl
+QED
+
+
+Definition parse_and_run_file_list_def:
+  parse_and_run_file_list lines fml Clist b =
+  case parse_lrup_one lines of
+    NONE => NONE
+  | SOME NONE => SOME fml
+  | SOME (SOME (step,rest)) =>
+    (case check_lrup_list step fml Clist b of
+      NONE => NONE
+    | SOME (fml', Clist', b') =>
+      parse_and_run_file_list rest fml' Clist' b')
+Termination
+  WF_REL_TAC` measure (LENGTH o FST)`>>
+  rw[]>>
+  drule parse_lrup_one_LENGTH>>
+  simp[]
+End
+
+Theorem parse_and_run_file_list_eq:
+  ∀lines fml Clist b.
+  parse_and_run_file_list lines fml Clist b =
+  case parse_lrups lines of
+    NONE => NONE
+  | SOME lrups => check_lrups_list lrups fml Clist b
+Proof
+  ho_match_mp_tac parse_and_run_file_list_ind>>
+  rw[]>>
+  simp[Once parse_and_run_file_list_def,Once parse_lrups_def]>>
+  every_case_tac>>
+  gvs[check_lrups_list_def]
+QED
+
+Quote add_cakeml:
+  fun check_unsat'' fd lno fml carr b =
+  case parse_lrup_one_arr lno fd of
+    None => fml
+  | Some step =>
+    (case check_lrup_arr lno step fml carr b of
+      (fml',carr',b') => check_unsat'' fd (lno+1) fml' carr' b')
+End
+
+Theorem check_unsat''_spec:
+  ∀lines fmlls Clist b fs fmlv fmllsv Carrv lno lnov bv.
+  NUM lno lnov ∧
+  LIST_REL (OPTION_TYPE vcclause_TYPE) fmlls fmllsv ∧
+  WORD8 b bv ∧
+  bnd_fml fmlls (LENGTH Clist)
+  ⇒
+  app (p : 'ffi ffi_proj)
+    ^(fetch_v "check_unsat''" (get_ml_prog_state()))
+    [fdv; lnov; fmlv; Carrv; bv]
+    (STDIO fs * ARRAY fmlv fmllsv *
+      W8ARRAY Carrv Clist * INSTREAM_LINES nulc fd fdv lines fs)
+    (POSTve
+      (λv.
+        SEP_EXISTS k fmllsv'.
+          STDIO (forwardFD fs fd k) *
+          INSTREAM_LINES nulc fd fdv [] (forwardFD fs fd k) *
+          ARRAY v fmllsv' *
+          &(unwrap_TYPE
+            (LIST_REL (OPTION_TYPE vcclause_TYPE))
+            (parse_and_run_file_list lines fmlls Clist b) fmllsv'))
+      (λe.
+        SEP_EXISTS k fmlv' fmllsv' lines'.
+          STDIO (forwardFD fs fd k) *
+          INSTREAM_LINES nulc fd fdv lines' (forwardFD fs fd k) *
+          ARRAY fmlv' fmllsv' *
+          &(Fail_exn e ∧
+            parse_and_run_file_list lines fmlls Clist b = NONE)))
+Proof
+  ho_match_mp_tac parse_and_run_file_list_ind>>
+  rpt strip_tac>>
+  xcf "check_unsat''" (get_ml_prog_state ())>>
+  simp[Once parse_and_run_file_list_def]>>
+  xlet `
+    POSTve
+      (λv.
+        SEP_EXISTS k lines'.
+          STDIO (forwardFD fs fd k) *
+          INSTREAM_LINES nulc fd fdv lines' (forwardFD fs fd k) *
+          ARRAY fmlv fmllsv * W8ARRAY Carrv Clist *
+          &(parse_lrup_one lines ≠ NONE ∧
+            OPTION_TYPE LRUP_LRUP_TYPE
+              (OPTION_MAP FST (THE (parse_lrup_one lines))) v ∧
+            (case THE (parse_lrup_one lines) of
+              NONE => lines' = []
+            | SOME res => lines' = SND res)))
+      (λe.
+        SEP_EXISTS k lines'.
+          STDIO (forwardFD fs fd k) *
+          INSTREAM_LINES nulc fd fdv lines' (forwardFD fs fd k) *
+          ARRAY fmlv fmllsv *
+          &(Fail_exn e ∧ parse_lrup_one lines = NONE))`
+  >- (
+    xapp>>
+    qexistsl_tac [`ARRAY fmlv fmllsv * W8ARRAY Carrv Clist`,`lines`,`fs`,
+      `fd`]>>
+    xsimpl>>
+    qexists_tac`lno`>>simp[]>>
+    rw[]>>
+    qexistsl_tac [`x`,`x'`]>>
+    xsimpl)
+  >- (
+    xsimpl>>rw[]>>
+    qexistsl_tac [`x`,`fmlv`,`fmllsv`,`x'`]>>
+    xsimpl>>
+    simp[Once parse_and_run_file_list_def])>>
+  Cases_on`parse_lrup_one lines`>>gvs[]>>
+  rename1`parse_lrup_one lines = SOME res`>>
+  Cases_on`res`>>gvs[OPTION_TYPE_def]
+  >- (
+    xmatch>>
+    xvar>>xsimpl>>
+    simp[unwrap_TYPE_def]>>
+    qexists_tac`k`>>xsimpl)>>
+  rename1`parse_lrup_one lines = SOME (SOME stp)`>>
+  Cases_on`stp`>>gvs[]>>
+  rename1`parse_lrup_one lines = SOME (SOME (step,rest))`>>
+  xmatch>>
+  xlet_auto
+  >- (
+    xsimpl>>rw[]>>
+    sep_triv)
+  >- (
+    xsimpl>>rw[]>>
+    qexistsl_tac [`k`,`fmlv`,`fmllsv`,`rest`]>>
+    xsimpl>>
+    simp[Once parse_and_run_file_list_def])>>
+  Cases_on`check_lrup_list step fmlls Clist b`>>gvs[]>>
+  rename1`check_lrup_list step fmlls Clist b = SOME res`>>
+  PairCases_on`res`>>gvs[]>>
+  xmatch>>
+  xlet_autop>>
+  xapp>>xsimpl>>
+  rpt(first_x_assum (irule_at Any))>>
+  qexistsl_tac [`forwardFD fs fd k`,`emp`]>>
+  xsimpl>>rw[]
+  >- (
+    simp[forwardFD_o]>>
+    sep_triv)>>
+  simp[forwardFD_o]>>
+  simp[Once parse_and_run_file_list_def]>>
+  xsimpl>>
+  sep_triv
+QED
+
+(*** The file-level entry point.
+
+  It takes the converted formula, so that its guarantee can be stated
+  on the formula the DIMACS file denotes rather than on the checker's
+  arrays.
+ ***)
+
+Quote add_cakeml:
+  fun check_unsat' vcfml fname n nc =
+  let
+    val fd = TextIO.openIn fname
+    val fml = build_fml_arr nc 1 vcfml
+    val carr = Word8Array.array n bw0
+    val chk = Inr (check_unsat'' fd 1 fml carr bw1)
+      handle Fail s => Inl s
+    val close = TextIO.closeIn fd;
+  in
+    case chk of
+      Inl s => Inl s
+    | Inr fml' => Inr (contains_emp_arr fml')
+  end
+  handle TextIO.BadFileName => Inl (notfound_string fname)
+End
+
+Theorem fastForwardFD_ADELKEY_same[simp]:
+  forwardFD fs fd n with infds updated_by ADELKEY fd =
+  fs with infds updated_by ADELKEY fd
+Proof
+  fs [forwardFD_def, IO_fs_component_equality]
+QED
+
+val bw0_v_thm = fetch "ccnf_arrayProg" "bw0_v_thm";
+val bw1_v_thm = fetch "ccnf_arrayProg" "bw1_v_thm";
+
+Theorem check_unsat'_spec:
+  NUM n nv ∧
+  NUM nc ncv ∧
+  LIST_TYPE vcclause_TYPE (conv_cfml cfml) vcfmlv ∧
+  FILENAME f fv ∧
+  hasFreeFD fs ∧
+  EVERY (EVERY nz_lit) cfml ∧
+  EVERY (EVERY (λl. var_lit l < n)) cfml
+  ⇒
+  app (p:'ffi ffi_proj) ^(fetch_v"check_unsat'"(get_ml_prog_state()))
+  [vcfmlv; fv; nv; ncv]
+  (STDIO fs)
+  (POSTv v.
+    STDIO fs *
+    SEP_EXISTS res.
+      &(SUM_TYPE STRING_TYPE BOOL res v ∧
+        (res = INR T ⇒ sols cfml = {})))
+Proof
+  rw[]>>
+  xcf"check_unsat'"(get_ml_prog_state ())>>
+  reverse (Cases_on `STD_streams fs`)
+  >- (fs [TextIOProofTheory.STDIO_def]>>xpull)>>
+  reverse (Cases_on`consistentFS fs`)
+  >- (fs [STDIO_def,IOFS_def,wfFS_def,consistentFS_def]>>xpull>>metis_tac[])>>
+  reverse (Cases_on `inFS_fname fs f`)>>simp[]
+  >- (
+    xhandle`POSTe ev.
+      &BadFileName_exn ev *
+      &(~inFS_fname fs f) *
+      STDIO fs`
+    >- (xlet_auto_spec (SOME openIn_STDIO_spec)>>xsimpl)>>
+    fs[BadFileName_exn_def]>>
+    xcases>>rw[]>>
+    xlet_auto>>xsimpl>>
+    xcon>>xsimpl>>
+    qexists_tac`INL (notfound_string f)`>>
+    simp[SUM_TYPE_def])>>
+  qmatch_goalsub_abbrev_tac`$POSTv Qval`>>
+  xhandle`$POSTv Qval`>>xsimpl>>
+  qunabbrev_tac`Qval`>>
+  xlet_auto_spec
+    (SOME (openIn_spec_lines |> Q.GEN `c0` |> Q.SPEC `nulc`))>>xsimpl>>
+  assume_tac bw0_v_thm>>
+  assume_tac bw1_v_thm>>
+  qmatch_goalsub_abbrev_tac`STDIO fss`>>
+  xlet_autop>>
+  xlet_autop>>
+  qabbrev_tac`fmlls = build_fml_list 1 (conv_cfml cfml) nc`>>
+  qabbrev_tac`Clist = REPLICATE n (0w:word8)`>>
+  `bnd_fml fmlls (LENGTH Clist)` by (
+    simp[Abbr`fmlls`,Abbr`Clist`]>>
+    irule bnd_fml_build_fml_list>>
+    irule bnd_clause_conv_cfml>>
+    fs[])>>
+  qabbrev_tac`lines = all_lines_file_gen nulc fs f`>>
+  xlet`POSTv resv.
+    SEP_EXISTS v0 fmllsv' fmlv' k rest.
+      STDIO (forwardFD fss (nextFD fs) k) *
+      INSTREAM_LINES nulc (nextFD fs) is rest (forwardFD fss (nextFD fs) k) *
+      ARRAY fmlv' fmllsv' *
+      &(
+      case parse_and_run_file_list lines fmlls Clist 1w of
+        NONE => resv = Conv (SOME (TypeStamp «Inl» 4)) [v0] ∧ ∃s. STRING_TYPE s v0
+      | SOME fmlls'' =>
+        resv = Conv (SOME (TypeStamp «Inr» 4)) [fmlv'] ∧
+        LIST_REL (OPTION_TYPE vcclause_TYPE) fmlls'' fmllsv'
+      )`
+  >- (
+    simp[]>>
+    TOP_CASE_TAC
+    >- (
+      xhandle`POSTe e.
+        SEP_EXISTS fmlv' fmllsv' rest k.
+          STDIO (forwardFD fss (nextFD fs) k) *
+          INSTREAM_LINES nulc (nextFD fs) is rest (forwardFD fss (nextFD fs) k) *
+          ARRAY fmlv' fmllsv' *
+          &(Fail_exn e ∧
+            parse_and_run_file_list lines fmlls Clist 1w = NONE)`
+      >- (
+        xlet`POSTe e.
+          SEP_EXISTS k fmlv' fmllsv' lines'.
+            STDIO (forwardFD fss (nextFD fs) k) *
+            INSTREAM_LINES nulc (nextFD fs) is lines'
+              (forwardFD fss (nextFD fs) k) *
+            ARRAY fmlv' fmllsv' *
+            &(Fail_exn e ∧
+              parse_and_run_file_list lines fmlls Clist 1w = NONE)`
+        >- (
+          xapp_spec check_unsat''_spec>>
+          xsimpl>>
+          rpt(first_x_assum (irule_at Any))>>
+          xsimpl>>
+          qexistsl_tac [`lines`,`fss`,`nextFD fs`,`emp`]>>
+          xsimpl>>
+          simp[Abbr`Clist`]>>
+          fs[unwrap_TYPE_def]>>
+          rw[]>>
+          sep_triv)>>
+        xsimpl>>rw[]>>
+        sep_triv)>>
+      fs[Fail_exn_def]>>
+      xcases>>
+      xcon>>xsimpl>>
+      simp[PULL_EXISTS]>>
+      asm_exists_tac>>simp[]>>
+      sep_triv)>>
+    xhandle`POSTv v.
+      SEP_EXISTS k rest fmllsv'.
+        STDIO (forwardFD fss (nextFD fs) k) *
+        INSTREAM_LINES nulc (nextFD fs) is rest (forwardFD fss (nextFD fs) k) *
+        (SEP_EXISTS fmlv'.
+          &(v = Conv (SOME (TypeStamp «Inr» 4)) [fmlv']) *
+          ARRAY fmlv' fmllsv') *
+        &(unwrap_TYPE
+          (LIST_REL (OPTION_TYPE vcclause_TYPE))
+          (parse_and_run_file_list lines fmlls Clist 1w) fmllsv')`
+    >- (
+      xlet`POSTv v.
+        SEP_EXISTS k fmllsv'.
+          STDIO (forwardFD fss (nextFD fs) k) *
+          INSTREAM_LINES nulc (nextFD fs) is [] (forwardFD fss (nextFD fs) k) *
+          ARRAY v fmllsv' *
+          &(unwrap_TYPE
+            (LIST_REL (OPTION_TYPE vcclause_TYPE))
+            (parse_and_run_file_list lines fmlls Clist 1w) fmllsv')`
+      >- (
+        xapp_spec check_unsat''_spec>>
+        xsimpl>>
+        rpt(first_x_assum (irule_at Any))>>
+        xsimpl>>
+        qexistsl_tac [`lines`,`fss`,`nextFD fs`,`emp`]>>
+        xsimpl>>
+        simp[Abbr`Clist`]>>
+        fs[unwrap_TYPE_def]>>
+        rw[]>>
+        sep_triv)>>
+      xcon>>xsimpl>>
+      sep_triv)>>
+    xsimpl>>
+    simp[unwrap_TYPE_def]>>
+    rw[]>>
+    sep_triv)>>
+  qspecl_then [`lines`,`fmlls`,`Clist`,`1w`]
+    strip_assume_tac parse_and_run_file_list_eq>>
+  gs[]>>
+  pop_assum kall_tac>>
+  xlet `POSTv v. STDIO fs * ARRAY fmlv' fmllsv'`
+  >- (
+    xapp_spec closeIn_spec_lines>>
+    rename [`ARRAY a1 a2`]>>
+    qexistsl_tac [`ARRAY a1 a2`,`rest`,`forwardFD fss (nextFD fs) k`,
+      `nextFD fs`,`nulc`]>>
+    conj_tac >- (
+      fs [forwardFD_def,Abbr`fss`]>>
+      imp_res_tac fsFFIPropsTheory.nextFD_ltX>>fs []>>
+      imp_res_tac fsFFIPropsTheory.STD_streams_nextFD>>fs [])>>
+    `validFileFD (nextFD fs) (forwardFD fss (nextFD fs) k).infds` by (
+      simp[validFileFD_forwardFD]>>simp[Abbr`fss`]>>
+      imp_res_tac fsFFIPropsTheory.nextFD_ltX>>fs []>>
+      match_mp_tac validFileFD_nextFD>>fs [])>>
+    xsimpl>>rw []>>
+    imp_res_tac (DECIDE ``n<m:num ==> n <= m``)>>
+    imp_res_tac fsFFIPropsTheory.nextFD_leX>>fs []>>
+    drule fsFFIPropsTheory.openFileFS_ADELKEY_nextFD>>
+    fs [Abbr`fss`]>>xsimpl)>>
+  Cases_on`parse_lrups lines`>>fs[]
+  >- (
+    xmatch>>
+    xcon>>xsimpl>>
+    qexists_tac`INL s`>>
+    simp[SUM_TYPE_def])>>
+  Cases_on`check_lrups_list x fmlls Clist 1w`>>fs[]
+  >- (
+    xmatch>>
+    xcon>>xsimpl>>
+    qexists_tac`INL s`>>
+    simp[SUM_TYPE_def])>>
+  xmatch>>
+  xlet_autop>>
+  xcon>>xsimpl>>
+  qexists_tac`INR (contains_emp_list x')`>>
+  simp[SUM_TYPE_def]>>
+  rw[]>>
+  irule check_lrups_unsat_list_sound>>
+  simp[check_lrups_unsat_list_def]>>
+  qexistsl_tac [`1`,`x`,`n`,`nc`]>>
+  gvs[Abbr`fmlls`,Abbr`Clist`]
+QED
+
+
+
+
+
+
+
+
+
+
+
+
+
+
