examples/cnf/lrup/README.md
@@ -1,0 +1,4 @@
+An LRUP checker
+
+[lrupScript.sml](lrupScript.sml):
+Basic specification of an LRUP checker
